remove cut of restore alts in And

code/rocq/valid_state.v
@@ -27,7 +27,7 @@ Module valid_state (U:Unif).
 
   Fixpoint base_and_ko s :=
     match s with
-    | And KO r r1 => (r == r1) && base_and_ko r1 (* should also say something about the program *)
+    | And KO r r1 => [&&base_and r, (cut r == r1) & base_and_ko r1] (* should also say something about the program *)
     | KO => true
     | _ => false
     end.
@@ -38,12 +38,12 @@ Module valid_state (U:Unif).
     | t => base_and_ko t
     end.
 
-  Definition base_or_ko s := 
+  (* Definition base_or_ko s := 
     match s with 
     | KO => true
     | Or KO _ t => base_or_aux_ko t
     | _ => false
-    end.
+    end. *)
 
   Fixpoint valid_state s :=
     match s with
@@ -52,7 +52,7 @@ Module valid_state (U:Unif).
     | Or Dead _ r => valid_state r
     | Or l _ r => valid_state l && (base_or_aux r || base_or_aux_ko r)
     | And l r0 r => 
-      valid_state l && (base_and r0 || base_and_ko r0) && if success l then valid_state r else (r0 == r)
+      [&& valid_state l, if success l then valid_state r else ((r0 == r) || (cut r0 == r)) & (base_and r0)]
     end.
 
   Lemma base_and_valid {A} : base_and A -> valid_state A.
@@ -102,19 +102,15 @@ Module valid_state (U:Unif).
   Qed.
 
   Lemma base_and_ko_valid {B}: base_and_ko B -> valid_state B.
-  Proof. by case: B => //= -[] //= A B /andP[]/eqP->->; rewrite eq_refl orbT. Qed.
-
-  Lemma base_and_base_and_ko_valid {B}:
-    base_and B || base_and_ko B -> valid_state B.
-  Proof. by move=> /orP []; [move=> /base_and_valid | move=> /base_and_ko_valid] => ->. Qed.
-
-  Lemma simpl_valid_state_and {A B0 B}: valid_state (And A B0 B) -> 
-    valid_state A /\ valid_state B /\ (base_and B0 || base_and_ko B0).
-  Proof. move=>/=/andP[]/andP[]//=> ->/[dup]/base_and_base_and_ko_valid + ->; case:success => // + /eqP <-//. Qed.
+  Proof.
+    elim: B => //.
+    by move=> []// HA B0 _ B HB/=/and3P[bB0 /eqP <-]; rewrite bB0 eqxx orbT.
+  Qed.
 
   Lemma simpl_valid_state_and1 {A B0 B}: valid_state (And A B0 B) -> 
-    valid_state A /\ base_and B0 || base_and_ko B0 /\ (if success A then valid_state B else B0 == B).
-  Proof. move=>/=/andP[]/andP[]// => ->/[dup]/base_and_base_and_ko_valid + ->; case:success => // + /eqP <-//. Qed.
+    valid_state A /\ (if success A then valid_state B else (B0 == B) || (cut B0 == B)) /\ base_and B0.
+  Proof. move=>/=/and3P[]// ->->->. Qed.
+
 
   Lemma base_or_ko_valid {B}: base_or_aux_ko B -> valid_state B.
   Proof.
@@ -122,12 +118,101 @@ Module valid_state (U:Unif).
     + move=> A HA s B HB /= /andP [] /base_and_ko_valid ->.
       move=> /[dup] /HB -> ->.
       by rewrite !orbT; destruct A.
-    + by move=> [] // HA B0 HB0 B HB /= /andP [] /[dup] /eqP -> _ ->; rewrite eq_refl orbT.
+    + by move=> [] // HA B0 _ B HB /= /and3P[] bB0 /eqP <-; rewrite eq_refl bB0 orbT.
   Qed.
+
 
   Lemma base_or_base_or_ko_valid {B}:
     base_or_aux B || base_or_aux_ko B -> valid_state B.
   Proof. by move=> /orP []; [move=> /base_or_valid | move=> /base_or_ko_valid] => ->. Qed.
+
+
+  Lemma base_and_base_and_ko_cut {B} : base_and B -> base_and_ko (cut B).
+  Proof. 
+    elim: B => // A + B + C /=.
+    case: A => //= _ _ _ HB HC /andP [] /eqP <- hB.
+    by rewrite hB (HB hB) eqxx.
+  Qed.
+
+  Lemma base_or_base_or_ko_cut {B}: base_or_aux B -> base_or_aux_ko (cut B).
+  Proof.
+    elim: B => //.
+    + by move=> A IHA s B IHB /= /andP [] /base_and_base_and_ko_cut -> /IHB ->.
+    + move=> [] //= _ _ _ B HB C HC /andP [] /eqP /[subst1] hC.
+      by rewrite eq_refl hC (base_and_base_and_ko_cut hC). 
+  Qed.
+
+  Lemma base_and_ko_cut {B}: base_and_ko B -> base_and_ko (cut B).
+  Proof.
+    elim: B => //.
+    move=> []// _ B _ C HC /= /and3P[] bB /eqP <-.
+    by rewrite cut_cut_same eqxx bB => ->.
+  Qed.
+  
+  Lemma base_or_ko_cut {B}: base_or_aux_ko B -> base_or_aux_ko (cut B).
+  Proof.
+    elim: B => //.
+      by move=> A HA s B HB /= /andP[]/base_and_ko_cut->/HB->.
+    move=> [] //= _ B0 _ B HB /and3P[] bB /eqP<-.
+    by rewrite cut_cut_same bB eqxx => ->.
+  Qed.
+
+  Lemma cut_dead1 {A}: cut A = dead A -> A = dead A.
+  Proof. by elim: A=> // A HA s B HB[]/=/HA<-/HB<-. Qed.
+
+  Lemma success_cut {A} : success (cut A) = success A.
+  Proof.
+    elim: A => //. 
+    + move=> A HA s B HB /=.
+      rewrite dead_cut_is_dead.
+      case: eqP.
+        move=> /cut_dead1//.
+        move=>->; rewrite dead_dead_same eq_refl//.
+      by case: eqP => //->; rewrite dead_dead_same cut_dead_is_dead.
+    + move=> A HA B HB C HC /=.
+      by rewrite HA HC.
+  Qed.
+
+  Lemma valid_state_cut {A}: valid_state A -> valid_state (cut A).
+  Proof.
+    elim: A => //.
+      move=> A HA s B HB/simpl_valid_state_or[].
+        by move=>[]->/=.
+      move=> [DA[VA bB]]/=.
+      rewrite (HA VA) (HB (base_or_base_or_ko_valid bB)).
+      move: bB => /orP[/base_or_base_or_ko_cut | /base_or_ko_cut]->; rewrite orbT; destruct A => //.
+    move=> A HA B0 _ B HB /=/and3P[] VA + bB0.
+    rewrite (HA VA) success_cut bB0 andbT/=.
+    case: ifP => // _/orP[].
+      by move=>/eqP->; rewrite eqxx orbT.
+    by move=>/eqP<-; rewrite cut_cut_same eqxx orbT.
+  Qed.
+
+  Lemma valid_state_compose_and {A2 B2 B02}: 
+    (if success A2 then valid_state B2 else ((B02 == B2) || (cut B02 == B2))) ->
+      base_and B02  ->
+        valid_state B2.
+  Proof. 
+    case: success => //.
+      move=>/orP[].
+        move=>/eqP->; apply: base_and_valid.
+      move=>/eqP<-/base_and_valid.
+      apply: valid_state_cut.  
+  Qed.
+  (* Lemma base_and_base_and_ko_valid {B}:
+    base_and B || base_and_ko B -> valid_state B.
+  Proof. by move=> /orP []; [move=> /base_and_valid | move=> /base_and_ko_valid] => ->. Qed. *)
+
+
+
+  Lemma simpl_valid_state_and {A B0 B}: valid_state (And A B0 B) -> 
+    valid_state A /\ valid_state B.
+  Proof.
+    move=>/= /and3P[]//=> ->; case:success => // /orP[]/eqP<-.
+      move=>/base_and_valid//.
+    by move=>/base_and_valid /valid_state_cut->.
+  Qed.
+
 
   Lemma valid_state_is_not_dead A: valid_state A -> A <> dead A.
   Proof. 
@@ -149,14 +234,14 @@ Module valid_state (U:Unif).
       move=> [].
         by move=> []+[]+[]+[]//.
       by move=> []+[]//; have:= (HA s1).
-    + move=> A HA B0 _ B HB s1 /simpl_valid_state_and[]/HA{}HA[]/HB{}HB _.
+    + move=> A HA B0 _ B HB s1 /simpl_valid_state_and[VA VB].
       move=>/simpl_expand_and_fail[].
-        by move=> []//; have:= HA s1.
+        by move=>[]; have:= HA s1 VA.
       move=> [].
         by move=> []+[]+[]//.
       move=> []s'[]A'[]B'[]H1[]H2.
       case: eqP => ///[subst1].
-      by have:= HB s'.
+      by have:= HB s' VB.
     Qed.
 
   Lemma success_dead {A}: success (dead A) = false.
@@ -170,40 +255,6 @@ Module valid_state (U:Unif).
     + by move=> ??; case F => //= -[] //=???; rewrite base_or_big_or_aux.
   Qed. 
 
-  Lemma base_and_base_and_ko_cut {B} : base_and B -> base_and_ko (cut B).
-  Proof. 
-    elim: B => // A + B + C /=.
-    case: A => //= _ _ _ HB HC /andP [] /eqP <- /HB.
-    by rewrite eq_refl.
-  Qed.
-
-
-  Lemma base_or_base_or_ko_cut {B}: base_or_aux B -> base_or_aux_ko (cut B).
-  Proof.
-    elim: B => //.
-    + by move=> A IHA s B IHB /= /andP [] /base_and_base_and_ko_cut -> /IHB ->.
-    + move=> [] //= _ _ _ B HB C HC /andP [] /eqP /[subst1].
-      by rewrite eq_refl => /base_and_base_and_ko_cut. 
-  Qed.
-
-  Lemma base_and_ko_cut {B}: base_and_ko B -> base_and_ko (cut B).
-  Proof.
-    elim: B => //.
-    move=> A HA B HB C HC /=; case: A HA => //= _ /andP [] /eqP <- /HB ->. 
-     by rewrite eq_refl.
-  Qed.
-  
-  Lemma base_or_ko_cut {B}: base_or_aux_ko B -> base_or_aux_ko (cut B).
-  Proof.
-    elim: B => //.
-      by move=> A HA s B HB /= /andP[]/base_and_ko_cut->/HB->.
-    move=> [] //= HA B0 HB0 B HB/andP[]/eqP/[subst1].
-    rewrite eq_refl.
-    apply: base_and_ko_cut.
-  Qed.
-
-  Lemma cut_dead1 {A}: cut A = dead A -> A = dead A.
-  Proof. by elim: A=> // A HA s B HB[]/=/HA<-/HB<-. Qed.
   
 
   Lemma expand_not_dead {s A r}: 
@@ -234,7 +285,7 @@ Module valid_state (U:Unif).
       + move=> s2 C /simpl_expand_or_solved [].
           move=> [A'[]] /HA{} => /(_ VA) /= H ->/=; congruence.
         move=> [B'[HA'[]]] /HB => /(_ (base_or_base_or_ko_valid VB)) /= + ->/=; congruence.
-    + move=> A HA B0 HB0 B HB s1 r /simpl_valid_state_and[]/[dup]VA/HA{}HA[]/[dup]VB/HB{}HB _.
+    + move=> A HA B0 HB0 B HB s1 r /simpl_valid_state_and[] VA VB.
       case: r.
       + move=> s2 C /simpl_expand_and_expanded [].
           by move=> [A'][] /HA H1 -> //.
@@ -243,12 +294,12 @@ Module valid_state (U:Unif).
           move=> [A'][] /HA /= + ->//.
         move=> [s'[A'[B'[]]]] /HA/= + [] _->//.
       + move=> C /simpl_expand_and_fail [].
-          by move=> []/HA//.
+          move=> [] H; have:= HA _ _ VA H => //.
         move=>[].
           by move=> [A'[DA[]]] /= + ->//.
-        move=> [s'[A'[B'[]]]]/HA/=+[]/HB/=.
-        case: ifP => /eqP ? + + ->; subst => /=; try congruence.
-      + move=> s2 C /simpl_expand_and_solved [s'[A'[B']]] []/HA.
+        move=> [s'[A'[B'[HA' [HB']]]]]->/=.
+        by case: ifP => /eqP?;subst => //; have:= HB _ _ VB HB'.
+      + move=> s2 C /simpl_expand_and_solved [s'[A'[B']]] [].
         by move=>/= + []/HB/= + <-.
   Qed.
 
@@ -269,7 +320,7 @@ Module valid_state (U:Unif).
         move=>/andP[]VA VB SA.
         have [A' H]:= HA s VA SA.
         by rewrite H; eexists.
-    + move=> A HA B0 HB0 B HB s /simpl_valid_state_and[VA[VB _]] /=/andP[SA SB].
+    + move=> A HA B0 HB0 B HB s /simpl_valid_state_and[] VA VB /=/andP[SA SB].
       have [A' H1]:= HA s VA SA; rewrite H1.
       have [B' H2]:= HB s VB SB; rewrite H2.
       by eexists.
@@ -289,8 +340,10 @@ Module valid_state (U:Unif).
       + move=> [A'[]]/= + [] /HB[] /= -> + -> /= => + ->.
         by have:= expand_failure_dead s1 VA.
     + move=> A HA B0 _ B HB s1 s2 C + /simpl_expand_and_solved [s3 [A' [B' ]]][]/HA{}HA[]/HB{}HB.
-      move=> /simpl_valid_state_and[]/HA []/= + + [] /HB[] + + _ <- /==> ->->->->.
-      repeat case: success => //.
+      move=> /simpl_valid_state_and[]VA VB <-/=.
+      have:= HA VA => -[]->->.
+      have:= HB VB => -[]->->.
+      do 2 case: success => //.
   Qed.
 
   Lemma expand_solved_success {s1 A s2 B}: valid_state A -> expand s1 A = Solved s2 B -> success A /\ success B.
@@ -305,8 +358,10 @@ Module valid_state (U:Unif).
         by move: VA => + _ H1; rewrite H1 valid_state_dead.
       move=> [B'[H1]].
       by have:= expand_failure_dead s1 VA.
-    + move=> A HA ? _ B HB s1 s2 C /simpl_valid_state_and[]/[dup]VA/HA{}HA[]/HB{}HB _.
-      by move=> /simpl_expand_and_solved [s3 [A' [B']]] [] /HA [] + + [] /HB [] + + <- /= => ->->->->.
+    + move=> A HA ? _ B HB s1 s2 C /simpl_valid_state_and[VA VB].
+      move=> /simpl_expand_and_solved [s3 [A' [B'[HA' [HB' <-]]]]]/=.
+      have:= HA _ _ _ VA HA' => -[] ->->.
+      by have:= HB _ _ _ VB HB' => -[] ->->.
   Qed.
 
   Lemma expand_failure_not_dead_right {s1 A B}: valid_state A -> expand s1 A = Failure B -> (A <> dead A) -> (B <> dead B).
@@ -335,19 +390,19 @@ Module valid_state (U:Unif).
       have: A <> dead A.
         move: VA => + H; rewrite H valid_state_dead//.
       move=> /HA//.
-    + move=> A HA B0 HB0 B HB C s1 /simpl_valid_state_and[]/[dup]VA/HA{}HA[]/[dup]VB/HB{}HB BB /simpl_expand_and_fail [].
+    + move=> A HA B0 HB0 B HB C s1 /simpl_valid_state_and[] VA VB /simpl_expand_and_fail [].
         move=> [] /HA{}HA.
         have: A <> dead A.
           by move: VA => + H; rewrite H valid_state_dead//.
-        move=> /HA//.
+        move=> /HA []//.
       move=> [].
         move=> [A'[DA[HA']]] -> //.
-      move=> [s'[A'[B'[]]]] + [] /HB{}HB.      
+      move=> [s'[A'[B'[HA' [HB' ->]]]]]/= _.
+      have H1 := HB _ _ VB HB'.
+      case: ifP => ///eqP/[subst1].
       have: B <> dead B.
         move: VB => + H; rewrite H valid_state_dead//.
-      move=> /HB{}HB + ->.
-      case: eqP => //=.
-        by move=> /[subst1]//.
+      by move=>/H1.
   Qed.
 
 
@@ -368,44 +423,21 @@ Module valid_state (U:Unif).
         move=> [B'[HD[+[+]]]]  /[subst1] /=.
         by move=> /HA [] -> _ /HB [] -> ->; rewrite if_same.
       by move=> [+[+]] /[subst1] /= => /HA [] -> _ /HB [] -> _; rewrite if_same.
-    + move=> A HA B0 _ B HB s C/simpl_valid_state_and[]/[dup]VA/HA{}HA[]/[dup]VB/HB{}HB BB.
+    + move=> A HA B0 _ B HB s C/simpl_valid_state_and[VA VB].
       move=> /simpl_expand_and_fail[].
-        by move=> [] /HA [] /= -> _ ->.
+        move=> [] HA' ->/=.
+        by have:= HA _ _ VA HA'=>-[]-> //.
       move=> [].
-        by move=> [?[A'[+]]]  /[subst1] /= /HA [] -> ->.
-      move=> [s' [A' [B' [+ [+]]]]] /[subst1] /=.
-      case: eqP.
-        by move: VA => /expand_solved_success{}HA -> /HA[] -> ? /HB[]->/=; rewrite orbT.
-      by move: VA => /expand_solved_success{}HA _/HA [] /= -> -> /HB [] -> ->; rewrite !orbT.
+        move=> [A'[DA'[HA' ->]]]/=.
+        by have:= HA _ _ VA HA' => -[]->->.
+      move=> [s' [A' [B' [HA' [HB' ->]]]]]/=.
+      have:= HB _ _ VB HB' => -[].
+      have:= expand_solved_success VA HA' => -[] ->.
+      case: ifP.
+        by move=>/eqP -> _ ->; rewrite orbT.
+      by move=> _ /= ->->->; rewrite !orbT.
   Qed. 
 
-  Lemma success_cut {A} : success A = success (cut A).
-  Proof.
-    elim: A => //. 
-    + move=> A HA s B HB /=.
-      rewrite dead_cut_is_dead.
-      case: eqP.
-        move=>->; rewrite cut_dead_is_dead dead_dead_same eq_refl//.
-      case: eqP.
-        move=> /cut_dead1//.
-      move=> //.
-    + move=> A HA B HB C HC /=.
-      by rewrite HA HC.
-  Qed.
-
-  Lemma valid_state_cut {A}: valid_state A -> valid_state (cut A).
-  Proof.
-    elim: A => //.
-      move=> A HA s B HB/simpl_valid_state_or[].
-        by move=>[]->/=.
-      move=> []/=DA[]/HA->/[dup] /base_or_base_or_ko_valid/HB->.
-      by move=> /orP[/base_or_base_or_ko_cut|/base_or_ko_cut] ->; rewrite orbT; case cut.
-    move=> A HA B0 HB0 B HB /=/andP[]/andP[]/HA -> H.
-    have: base_and_ko (cut B0).
-      move: H => /orP [/base_and_base_and_ko_cut|/base_and_ko_cut] //.
-    move=>->; rewrite orbT -success_cut.
-    by case: success => ///eqP->; rewrite eq_refl.
-  Qed.
 
   Lemma valid_state_expand {s A r}:
     expand s A = r -> valid_state A -> valid_state (get_state r).
@@ -447,34 +479,46 @@ Module valid_state (U:Unif).
             + move=> [B'[HA'[HB']]] /[subst1] /simpl_valid_state_or [][].
               + by move=> /[subst1] VB /=; rewrite (IHB _ _ HB' VB).
               + by move=> DA [] VA /base_or_base_or_ko_valid /= VB; rewrite (IHB _ _ HB' VB).
-    + move=> A IHA B0 HB0 B IHB s1 [].
+    + move=> A HA B0 _ B HB s1 [].
       + move=> s2 C => /simpl_expand_and_expanded [].
-          move=> [A'[HA']] /[subst1] /=/andP [] /andP [] VA /[dup] /base_and_base_and_ko_valid VB0.
-          rewrite (IHA _ _ HA' VA) => /[dup]+->/=.
-            case SA: success.
-              have:= succes_is_solved s1 VA SA; rewrite HA' => -[?] //.
-            by move=> _ /eqP /[subst1]; rewrite VB0 eq_refl if_same.
-        move=> [s[A'[B']]] [] /[dup] /expand_solved_success H1 /IHA{}IHA[]/IHB{}IHB /[subst1].
-        move=> /simpl_valid_state_and[] /[dup]/expand_solved_success H /[dup].
-        by move=> /H1 [] /= _ -> /IHA /= -> []/IHB-> ->.
-      + move=> s2 C /simpl_expand_and_cut [].
-          move=> [A' [HA']] /[subst1] /= /andP [] /andP [] /[dup] VA /(IHA _ _ HA') -> /[dup] /base_and_base_and_ko_valid H ->.
-          case SA: success.
+          move=> [A'[HA' ->]] /simpl_valid_state_and1 [VA [VB bB0]]/=.
+          rewrite (HA _ _ HA' VA) bB0 (valid_state_compose_and VB bB0).
+          move: VB; case SA: success.
             have:= succes_is_solved s1 VA SA; rewrite HA' => -[?] //.
-          move=> /eqP /[subst1]; rewrite H eq_refl; case: success => //.
-        move=> [s'[A'[B']]] [] + [] + -> /simpl_valid_state_and1 [] /[dup]VA/IHA {}IHA [] /[dup] /= /base_and_base_and_ko_valid /HB0{}HB0 ->.
-        by rewrite -!success_cut => /[dup]/(expand_solved_success VA)[]->-> /IHA/valid_state_cut-> /IHB{}IHB/IHB->.
+          by move=>->; rewrite if_same.
+        move=> [s[A'[B'[HA'[HB' ->]]]]].
+        move=> /simpl_valid_state_and1 [VA].
+        have:= expand_solved_success VA HA' => -[]/=->->[] VB ->.
+        by rewrite (HA _ _ HA' VA) (HB _ _ HB' VB).
+      + move=> s2 C /simpl_expand_and_cut [].
+          move=> [A' [HA' ->]] /simpl_valid_state_and1[VA [VB bB0]]/=.
+          rewrite (HA _ _ HA' VA) bB0 (valid_state_compose_and VB bB0).
+          move: VB; case SA: success.
+            have:= succes_is_solved s1 VA SA; rewrite HA' => -[?] //.
+          by move=>->; rewrite if_same.
+        move=> [s'[A'[B'[HA'[HB' ->]]]]]/simpl_valid_state_and1[VA [VB bB0]]/=.
+        move: VB.
+        have:= expand_solved_success VA HA' => -[] -> sA' VB.
+        by rewrite (HB _ _ HB' VB) success_cut bB0 sA' (valid_state_cut (HA _ _ HA' VA)).
       + move=> s2 /simpl_expand_and_fail [].
           by move=> [] /expand_failure_dead H _ /simpl_valid_state_and1 [] /H.
         move=> [].
-          move=> [DA'[A']] [] /[dup] HH /IHA{}IHA /[subst1] /=/andP [] /andP[] /[dup] /IHA -> + ->.
-          move: HH => /expand_failure_failed{}HA/HA[] /failed_success->/failed_success->->//.
-        move=> [s'[A'[B'[HA'[HB']]]]] /[subst1] /simpl_valid_state_and [] /[dup] + /(IHA _ _ HA')/= + [].
-        move: HA' => /expand_solved_success H1 /H1[] _.
-        move: HB' => /IHB{}IHB + + /IHB.
-        by case: eqP => [->|]//= _ ->->->->.
-      + move=> s C /simpl_expand_and_solved [s'[A'[B'[]]]] /[dup]/expand_solved_success H. 
-        by move=> /IHA{}IHA [] /IHB{}IHB<- /simpl_valid_state_and [] /[dup] /H []/= _ -> /IHA -> []/IHB/= ->->.
+          move=> [A'[DA'[HA' ->]]] /simpl_valid_state_and1 [VA[VB bB0]] /=.
+          rewrite (HA _ _ HA' VA) bB0.
+          move: VB.
+          have:= expand_failure_failed VA HA' => -[].
+          do 2 move=> /failed_success->.
+          by move=>->.
+        move=> [s'[A'[B'[HA'[HB' ->]]]]] /simpl_valid_state_and1 [VA [VB bB0]]/=.
+        have:= HA _ _ HA' VA.
+        have:= HB _ _ HB' (valid_state_compose_and VB bB0).
+        move=>/=.
+        case: ifP => [/eqP->|]// _ /=->->.
+        by have:= expand_solved_success VA HA' => -[] _ ->.
+      + move=> s C /simpl_expand_and_solved [s'[A'[B'[HA' [HB'<-]]]]].
+        move=> /simpl_valid_state_and1 [VA [+ bB0]].
+        have:= expand_solved_success VA HA' => /= -[] ->-> VB.
+        by rewrite (HA _ _ HA' VA) (HB _ _ HB' VB) bB0.
   Qed.
 
   Lemma expand_failure_not_dead_left {s1 A B}: valid_state A -> expand s1 A = Failure B -> B <> Dead -> A <> dead A.
@@ -532,11 +576,28 @@ Module valid_state (U:Unif).
      base_and A || base_and_ko A ->  next_alt_aux true s1 A = Some (s2, B) -> A = B.
   Proof.
     elim: A s1 s2 B => //; move=> [] //.
-    + move=> _ B0 HB0 B HB s1 s2 C /= /andP [] /eqP /[subst1] BA.
+    + move=> _ B0 _ B HB s1 s2 C /= /and3P[] bB0 /eqP cB0 bcB0.
       case NB: next_alt_aux => // [[ ]] [] /[subst2].
-      rewrite BA in HB.
-      by rewrite (HB _ _ _ _ NB)//orbT.
+      by have:= HB _ _ _ _ NB; rewrite bcB0 orbT => /(_ isT) <-.
     + move=> p a _ B0 HB0 B HB s1 s2 C /= /orP []// /andP []/eqP/[subst1] BB.
+      case NB: next_alt_aux => // [[ ]] [] /[subst2].
+      by rewrite BB in HB; rewrite (HB _ _ _ isT NB).
+  Qed.
+
+  Lemma next_alt_aux_base_and1 {s1 s2 A B}:
+     base_and A ->  next_alt_aux true s1 A = Some (s2, B) -> A = B.
+  Proof.
+    elim: A s1 s2 B => //; move=> [] //.
+    + move=> p a _ B0 HB0 B HB s1 s2 C /= /andP []/eqP/[subst1] BB.
+      case NB: next_alt_aux => // [[ ]] [] /[subst2].
+      by rewrite BB in HB; rewrite (HB _ _ _ isT NB).
+  Qed.
+
+  Lemma next_alt_aux_base_and2 {s1 s2 A B}:
+     base_and A ->  next_alt_aux true s1 (cut A) = Some (s2, B) -> cut A = B.
+  Proof.
+    elim: A s1 s2 B => //; move=> [] //.
+    + move=> p a _ B0 HB0 B HB s1 s2 C /= /andP []/eqP/[subst1] BB.
       case NB: next_alt_aux => // [[ ]] [] /[subst2].
       by rewrite BB in HB; rewrite (HB _ _ _ isT NB).
   Qed.
@@ -556,19 +617,16 @@ Module valid_state (U:Unif).
         + by move=> [B'[?[+]]] /[subst1] => /HB /= ->.
         + by move=> [A'[_ [+]]] /[subst1] /HA /= ->; rewrite VB VBa; destruct A'.
         + by move=> [_ [NA]] /[subst1] /=.
-    + move=> A HA B0 HB0 B HB b s1 s2 C.
-      move=> /= /andP [] /andP [] VA /[dup] /base_and_base_and_ko_valid VB0 BB.
-      case SA: success.
-      + move=> VB.
-        case NB: next_alt_aux => [[ ]|].
-        + by move=> [] /[subst2] /= ; rewrite VA (HB _ _ _ _ VB NB) BB SA.
-        + case NA: next_alt_aux => [[ ]|] // [] /[subst2] /=.
-           by rewrite (HA _ _ _ _ VA NA) BB eq_refl VB0 if_same.
-      + move=> /eqP /[subst1].
-        case NB: next_alt_aux => [[s3 D]|].
-        + by move=> [] /[subst2] /=; rewrite SA VA BB (next_alt_aux_base_and BB NB) eq_refl.
-        + case NA: next_alt_aux => // [[ ]] [] /[subst2] /=.
-          by rewrite (HA _ _ _ _ VA NA) eq_refl BB VB0 if_same.
+    + move=> A HA B0 HB0 B HB b s1 s2 C /simpl_valid_state_and1 [VA [VB bB0]]/=.
+      case NB: next_alt_aux => [[s3 D]|].
+        move=> [] /[subst2] /=; rewrite VA bB0.
+        have VD:= (HB _ _ _ _ (valid_state_compose_and VB bB0) NB).
+        rewrite VD.
+        move: VB; case: success => ///orP[]/eqP/[subst1].
+          by have:= next_alt_aux_base_and1 bB0 NB=>->; rewrite eqxx.
+        by have:= next_alt_aux_base_and2 bB0 NB=>->; rewrite eqxx orbT.
+      case NA: next_alt_aux => // [[s3 D]] [] /[subst2] /=.
+      by rewrite (HA _ _ _ _ VA NA) eqxx bB0 (base_and_valid bB0) if_same.
   Qed.
 
   Lemma valid_state_next_alt {s s' A B} : 
