code/rocq/lang.v
@@ -198,7 +198,7 @@ Module Run (U : Unif).
       se dovesse lanciare D la seconda volta, mi ritrovo con (KO, D) che 
       è spiacevole...
     *)
-    | And A B0 B => And (cut A) (cut B0) (cut B)
+    | And A B0 B => And (cut A) B0 (cut B)
     | Or A s B => Or (cut A) s (cut B)
     end.
 
@@ -528,7 +528,7 @@ Module Run (U : Unif).
     + move=> A HA B0 HB0 B HB.
 
       (* case X: eq_op => //=. *)
-      by move=> /=; rewrite HA HB0 HB.
+      by move=> /=; rewrite HA ?HB0 HB.
       (* case Y: eq_op => //=.
       exfalso.
       by move: Y X => /eqP [] /cut_dead ->; rewrite eq_refl. *)
